rocq-osiris/theories/program_logic/program_logic.v
@@ -1,7 +1,7 @@
 (* This file summarizes the content of program_logic/ directory. *)
 
 Require Export
-  thread_step
+  subjective_step
   ewp
   triples
   stop_rules
